working on the Refinement proof and BTree boiler plate definitions

Splinter/BTree.i.dfy
@@ -7,11 +7,19 @@ include "SplinterTree.i.dfy"
 include "Message.s.dfy"
 include "Interp.s.dfy"
 
+/*
+
+  In our splinter datastructure there's two possible things that could be btrees
+  The current branch in the membuffer (fully in memory -- but we can asynchronously persist the working branch to disk) and the branch trees in the splinter tree on disk
+
+  Incorporation : Process of updating the splinter tree pointers such that the current branch (is persisted on disk) and added to the splinter tree root
+
+*/
 abstract module BtreeModel {
   type Key = Keys.Element
   type Value
 
-
+  datatype BtreeState = Active | Frozen;
   datatype NodeState = None | OnDisk; // Might need arguments ???
 
   // Node in the btree
@@ -19,9 +27,9 @@ abstract module BtreeModel {
   // pivots to provide an ordering of the children
   datatype Node =
     | Leaf(linear keys: seq<Key>, values: seq<Value>, state: NodeState)
-    | Index(linear pivots: seq<Key>, children: lseq<Node>)
+    | Index(linear pivots: seq<Key>, children: lseq<Node>, state: NodeState)
 
-
+  datatype Variables = Variables(root : Node, state: BtreeState)
 
 
 }
